Support formal circuits in witness compiler

Clean/Examples/Witness.lean
@@ -1,4 +1,5 @@
 import Clean.Circuit
+import Clean.Circomlib.Gates
 import Clean.Utils.Primes
 
 namespace Examples.Witness
@@ -25,9 +26,49 @@ def vectorWitness : Circuit Rat (Vector (Expression Rat) 3) := do
 
 compile_witness vectorWitness => vectorWitnessCompiled
 
-compile_witness do
-    let x : Expression (F pBabybear) := .const 0
-    assertZero (x * (x - 1))
-  => babybearZeroOneWitness
+
+def formalBaseWitness : FormalCircuitBase Rat field field where
+  main x := do
+    let y ← witnessField fun env => env x + 1
+    assertZero (y - (x + 1))
+    return y
+
+compile_witness formalBaseWitness => formalBaseWitnessCompiled
+
+compile_witness (Circomlib.AND.circuit (p:=pBabybear)) => circomlibAndWitness
+compile_witness (Circomlib.XOR.circuit (p:=pBabybear)) => circomlibXorWitness
+compile_witness (Circomlib.OR.circuit (p:=pBabybear)) => circomlibOrWitness
+
+@[circuit_norm]
+def assertBoolWithReturn : FormalAssertion (F pBabybear) field where
+  -- works
+  main x := do assertZero (x * (x - 1)); return ()
+  -- doesn't work
+  -- main x := assertZero (x * (x - 1))
+  Spec x := IsBool x
+  soundness := by circuit_proof_all
+  completeness := by circuit_proof_all
+
+
+example : ∀ a : Expression (F pBabybear) × Expression (F pBabybear),
+  ExplicitCircuit (Circomlib.AND.circuit.main a) := by infer_explicit_circuit
+
+/-- error: unsolved goals
+a✝ : Expression (F pBabybear)
+⊢ ExplicitCircuit (assertBool.main a✝) -/
+#guard_msgs in
+example : ∀ a : Expression (F pBabybear), ExplicitCircuit (assertBool.main a) := by
+  infer_explicit_circuit
+
+example : ∀ a : Expression (F pBabybear),
+  ExplicitCircuit ((fun x => assertZero (x * (x - 1)) : Var field (F pBabybear) → Circuit (F pBabybear) (Var unit (F pBabybear))) a) := by
+  infer_explicit_circuit
+
+example : ∀ a : Expression (F pBabybear), ExplicitCircuit (assertBoolWithReturn.main a) := by
+  infer_explicit_circuit
+
+compile_witness (assertBool (p:=pBabybear)) => assertBoolWitness
+
+compile_witness assertBoolWithReturn => assertBoolWithReturnWitness
 
 end Examples.Witness
